updated normal form proof and statement: due to generalized rule, pat-compl. alg. now reaches FVF

thys/Pattern_Completeness/Pattern_Completeness_Multiset.thy
@@ -133,11 +133,17 @@ definition weak_finite_var_form_mp :: "('f,'v,'s)match_problem_mset \<Rightarrow
           (\<exists> x. (Var x, Var y) \<in># mp \<and> inf_sort (snd x))
         \<and> (\<forall> t. (t, Var y) \<in># mp \<longrightarrow> root t \<in> {None, Some (f,length ts)})))"
 
+definition finite_var_form_mp :: "('f,'v,'s)match_problem_mset \<Rightarrow> bool" where
+  "finite_var_form_mp mp = (\<forall> (t,l) \<in># mp. \<exists> x y. t = Var x \<and> l = Var y \<and> \<not> inf_sort (snd x))" 
+
 definition weak_finite_var_form_pp :: "('f,'v,'s)pat_problem_mset \<Rightarrow> bool" where
   "weak_finite_var_form_pp p = (\<forall> mp \<in># p. weak_finite_var_form_mp mp)" 
 
-lemma pat_fail_or_trans_or_weak_finite_var_form: assumes "improved \<Longrightarrow> infinite (UNIV :: 'v set)" 
-  shows "pat_fail p \<or> (\<exists> ps. p \<Rightarrow>\<^sub>m ps) \<or> (improved \<and> weak_finite_var_form_pp p)" 
+definition finite_var_form_pp :: "('f,'v,'s)pat_problem_mset \<Rightarrow> bool" where
+  "finite_var_form_pp p = (\<forall> mp \<in># p. finite_var_form_mp mp)" 
+
+lemma pat_fail_or_trans_or_finite_var_form: assumes "improved \<Longrightarrow> infinite (UNIV :: 'v set)" 
+  shows "pat_fail p \<or> (\<exists> ps. p \<Rightarrow>\<^sub>m ps) \<or> (improved \<and> finite_var_form_pp p)" 
 proof (cases "p = {#}")
   case True
   with pat_empty show ?thesis by auto
@@ -234,11 +240,10 @@ next
               show ?thesis using y conf not_impr by auto
             next
               case impr: True
-              show ?thesis
+              (* we first prove that we can reach weak-finite-var-form and switch to finite-var-form later *)
+              (* TODO: one might clean up this two-way proof and directly go to finite-var-form *)
+              have "(pat_fail p \<or> (\<exists>ps. p \<Rightarrow>\<^sub>m ps)) \<or> weak_finite_var_form_pp p" 
               proof (cases "weak_finite_var_form_pp p")
-                case True
-                with impr show ?thesis by auto
-              next
                 case False
                 from this[unfolded weak_finite_var_form_pp_def] obtain mp 
                   where mp: "mp \<in># p" and nmp: "\<not> weak_finite_var_form_mp mp" by auto
@@ -328,7 +333,81 @@ next
                     from pat_simp_mp[OF this, of p'] p' show ?thesis by auto
                   qed
                 qed
-              qed
+              qed auto
+              (* and continue to switch from weak-finite-var-form to full finite-var-form *)
+              thus ?thesis
+              proof (elim context_disjE)
+                assume no_step: "\<not> (pat_fail p \<or> (\<exists>ps. p \<Rightarrow>\<^sub>m ps))" 
+                assume "weak_finite_var_form_pp p" 
+                note wfvf = this[unfolded weak_finite_var_form_pp_def weak_finite_var_form_mp_def, rule_format]
+                note get_var = wfvf[THEN conjunct1, rule_format]
+                note fun_case = wfvf[THEN conjunct2, rule_format]
+                (* fin-predicate: all variables in mp are of finite sort *)
+                define fin where "fin mp = Ball (tvars_mp (mp_mset mp)) (\<lambda> x. \<not> inf_sort (snd x))" for mp
+                define p_fin where "p_fin = filter_mset fin p" 
+                define p_inf where "p_inf = filter_mset (Not o fin) p" 
+                have p_split: "p = p_inf + p_fin" unfolding p_fin_def p_inf_def by auto
+                show ?thesis
+                proof (cases "p_inf = {#}")
+                  case True
+                  have fin: "\<And> mp. mp \<in># p \<Longrightarrow> fin mp" unfolding p_split True unfolding p_fin_def by auto
+                  have "finite_var_form_pp p" 
+                    unfolding finite_var_form_pp_def finite_var_form_mp_def
+                  proof (intro ballI, clarify)
+                    fix mp t l
+                    assume mp: "mp \<in># p" and tl: "(t,l) \<in># mp" 
+                    from fin[OF mp, unfolded fin_def tvars_mp_def] tl 
+                    have fint: "\<And> x. x \<in> vars t \<Longrightarrow> \<not> inf_sort (snd x)" by auto
+                    from get_var[OF mp tl] tl obtain y where 
+                      ty: "(t, Var y) \<in># mp" and ly: "l = Var y" by (cases l, auto)
+                    have "is_Var t"
+                    proof (cases t)
+                      case (Fun f ts)
+                      with ty have "(Fun f ts, Var y) \<in># mp" by auto
+                      from fun_case[OF mp this] obtain x where "(Var x, Var y) \<in># mp" "inf_sort (snd x)" by auto
+                      with fin[OF mp, unfolded fin_def tvars_mp_def] tl have False by auto
+                      thus ?thesis by auto
+                    qed auto
+                    then obtain x where tx: "t = Var x" by auto
+                    from fint[unfolded tx] have fin: "\<not> inf_sort (snd x)" by auto
+                    with ly tx show "\<exists>x y. t = Var x \<and> l = Var y \<and> \<not> inf_sort (snd x)" by auto
+                  qed
+                  with impr show ?thesis by auto
+                next
+                  case False
+                  have "\<forall>x\<in>tvars_pp (pat_mset p_fin). \<not> inf_sort (snd x)" unfolding p_fin_def fin_def
+                    by (auto simp: tvars_pp_def)
+                  from pat_inf_var_conflict[OF _ False this, folded p_split] no_step
+                  obtain mp where mp: "mp \<in># p" and inf: "\<not> fin mp" and no_confl: "\<not> inf_var_conflict (mp_mset mp)" 
+                    unfolding p_inf_def by fastforce
+                  from inf[unfolded fin_def tvars_mp_def]
+                  obtain t l x where tl: "(t,l) \<in># mp" and x: "x \<in> vars t" and inf: "inf_sort (snd x)" by auto
+                  from get_var[OF mp tl] tl obtain y where ty: "(t, Var y) \<in># mp" by auto
+                  have "\<exists> x. (Var x, Var y) \<in># mp \<and> inf_sort (snd x)" 
+                  proof (cases t)
+                    case (Var z)
+                    with ty inf x show ?thesis by (intro exI[of _ z], auto)
+                  next
+                    case (Fun f ts)
+                    from fun_case[OF mp ty[unfolded Fun]] show ?thesis by auto
+                  qed
+                  then obtain x where xy: "(Var x, Var y) \<in># mp" and inf: "inf_sort (snd x)" by auto
+                  from mset_add[OF xy] obtain mp' where mp': "mp = add_mset (Var x, Var y) mp'" by auto
+                  from nsvar[simplified, rule_format, OF mp[unfolded mp']] obtain s y' where 
+                    sy': "(s,y') \<in># mp'" and y': "y \<in> vars y'" by force
+                  from mset_add[OF sy'] mp' obtain mp'' where 
+                    mp'': "mp = add_mset (s,y') (add_mset (Var x, Var y) mp'')" 
+                    by auto
+                  from get_var[OF mp[unfolded mp'']] y'
+                  have mp'': "mp = add_mset (s, Var y) (add_mset (Var x, Var y) mp'')" 
+                    unfolding mp'' by (cases y', auto)
+                  from ndup mp'' mp have sx: "s \<noteq> Var x" by auto
+                  from no_confl[unfolded inf_var_conflict_def not_ex, rule_format, of s y "Var x" x] mp'' inf                     
+                  have "\<not> Conflict_Var s (Var x) x" by auto
+                  with sx have False by (cases s, auto simp: conflicts.simps)
+                  thus ?thesis by auto
+                qed
+              qed auto
             qed
           next
             case no_non_inf: False
@@ -361,7 +440,7 @@ context
 begin
   
 lemma pat_fail_or_trans: "pat_fail p \<or> (\<exists> ps. p \<Rightarrow>\<^sub>m ps)" 
-  using pat_fail_or_trans_or_weak_finite_var_form[of p] non_improved by auto
+  using pat_fail_or_trans_or_finite_var_form[of p] non_improved by auto
 
 text \<open>Pattern problems just have two normal forms: 
   empty set (solvable) or bottom (not solvable)\<close>
@@ -380,6 +459,35 @@ proof (rule ccontr)
   from P_failure[OF this, of P', folded P] nNF NF show False by auto
 qed
 end
+
+
+context
+  assumes improved: "improved"
+    and inf: "infinite (UNIV :: 'v set)" 
+begin
+  
+lemma pat_fail_or_trans_or_fvf: "pat_fail p \<or> (\<exists> ps. p \<Rightarrow>\<^sub>m ps) \<or> finite_var_form_pp p" 
+  using pat_fail_or_trans_or_finite_var_form[of p, OF inf] by auto
+
+text \<open>Normal forms only consist of finite-var-form pattern problems\<close>
+theorem P_step_NF_fvf: 
+  assumes NF: "P \<in> NF \<Rrightarrow>" 
+    and p: "p \<in># P"
+  shows "finite_var_form_pp p"  
+proof (rule ccontr)
+  assume nfvf: "\<not> ?thesis" 
+  from mset_add[OF p] obtain P' where P: "P = add_mset p P'" by auto
+  from NF have NF: "\<not> (\<exists> Q. P \<Rrightarrow>\<^sub>m Q)" unfolding P_step_def by blast
+  from pat_fail_or_trans_or_fvf[of p] nfvf
+  obtain ps where "pat_fail p \<or> p \<Rightarrow>\<^sub>m ps" by auto
+  with P_simp_pp[of p ps] NF
+  have "pat_fail p" unfolding P by auto
+  from P_failure[OF this, of P', folded P] NF have "P = {# {#} #}" by auto
+  with P have "p = {#}" by auto
+  with nfvf show False unfolding finite_var_form_pp_def by auto
+qed
+end
+
 end
 
 subsection \<open>Termination\<close>
